Finish verifying eio/rcfd.

theories/eio/rcfd.v
@@ -1,7 +1,9 @@
 From heap_lang Require Import
   prelude.
+From heap_lang.common Require Import
+  gmultiset.
 From heap_lang.iris.base_logic Require Import
-  lib.auth_dgset
+  lib.auth_gmultiset
   lib.mono_state.
 From heap_lang.language Require Import
   tactics
@@ -17,9 +19,9 @@ From heap_lang.eio Require Import
 Implicit Types b : bool.
 Implicit Types ops : Z.
 Implicit Types q : Qp.
-Implicit Types qs : gset Qp.
+Implicit Types qs : gmultiset Qp.
 Implicit Types l l_state : loc.
-Implicit Types t v fd state fn : val.
+Implicit Types t v v_state fd fn : val.
 
 #[local] Definition state_match : val :=
   λ: "state" "Open" "Closing",
@@ -115,6 +117,30 @@ Qed.
 #[global] Opaque state_Closing.
 #[global] Opaque ClosingV.
 
+Inductive rcfd_state :=
+  | RcfdStateOpen fd
+  | RcfdStateClosing fn.
+Implicit Types state : rcfd_state.
+
+#[local] Instance rcfd_state_inhabited : Inhabited rcfd_state :=
+  populate (RcfdStateOpen inhabitant).
+
+#[local] Definition state_to_val state :=
+  match state with
+  | RcfdStateOpen fd =>
+      &&Open fd
+  | RcfdStateClosing fn =>
+      &&Closing fn
+  end.
+#[local] Arguments state_to_val !_ / : assert.
+#[local] Coercion state_to_val : rcfd_state >-> val.
+
+#[local] Instance state_to_val_inj :
+  Inj (=) (=) state_to_val.
+Proof.
+  intros [] []; naive_solver.
+Qed.
+
 #[local] Notation "t '.[ops]'" :=
   t.[0]%stdpp
 ( at level 5
@@ -140,7 +166,7 @@ Definition rcfd_make : val :=
   λ: <>,
     ref (&Closing (λ: <>, #())).
 
-Definition rcfd_put : val :=
+#[local] Definition rcfd_put : val :=
   λ: "t",
     let: "old" := FAA "t".[ops] #-1 in
     if: "old" = #1 then (
@@ -177,13 +203,14 @@ Definition rcfd_close : val :=
     let: "prev" := !"t".[fd] in
     match: !"prev" with
     | Open "fd" =>
-        let: "next" := &Closing (λ: <>, unix_close "fd") in
+        let: "close" := λ: <>, unix_close "fd" in
+        let: "next" := ref (&Closing "close") in
         if: CAS "t".[fd] "prev" "next" then (
-          if: !"t".[ops] = #0 && CAS "t".[fd] "next" (rcfd_fully_closed #()) then (
-            unix_close "fd"
+          (if: (!"t".[ops] = #0) && CAS "t".[fd] "next" (rcfd_fully_closed #()) then (
+            "close" #()
           ) else (
             #()
-          ) ;;
+          )) ;;
           #true
         ) else (
           #false
@@ -240,12 +267,12 @@ Inductive rcfd_lstep : relation rcfd_lstate :=
 #[local] Hint Constructors rcfd_lstep : core.
 
 Class RcfdG Σ `{heap_GS : !heapGS Σ} := {
-  #[local] rcfd_G_tokens_G :: AuthDgsetG Σ Qp ;
+  #[local] rcfd_G_tokens_G :: AuthGmultisetG Σ Qp ;
   #[local] rcfd_G_lstate_G :: MonoStateG rcfd_lstep Σ ;
 }.
 
 Definition rcfd_Σ := #[
-  auth_dgset_Σ Qp ;
+  auth_gmultiset_Σ Qp ;
   mono_state_Σ rcfd_lstep
 ].
 #[global] Instance subG_rcfd_Σ `{heap_GS : !heapGS Σ} :
@@ -281,11 +308,11 @@ Section rcfd_G.
   Qed.
 
   #[local] Definition rcfd_tokens_auth' γ_tokens qs :=
-    auth_dgset_auth γ_tokens (DfracOwn 1) qs.
+    auth_gmultiset_auth γ_tokens (DfracOwn 1) qs.
   #[local] Definition rcfd_tokens_auth γ qs :=
     rcfd_tokens_auth' γ.(rcfd_name_tokens) qs.
   #[local] Definition rcfd_tokens_frag' γ_tokens q :=
-    auth_dgset_frag γ_tokens {[q]}.
+    auth_gmultiset_frag γ_tokens {[+q+]}.
   #[local] Definition rcfd_tokens_frag γ q :=
     rcfd_tokens_frag' γ.(rcfd_name_tokens) q.
 
@@ -299,25 +326,25 @@ Section rcfd_G.
     rcfd_lstate_lb' γ.(rcfd_name_lstate) lstate.
 
   #[local] Definition rcfd_inv_inner l γ fd chars : iProp Σ :=
-    ∃ ops l_state state lstate,
+    ∃ state lstate ops l_state,
     l.[ops] ↦ #ops ∗
-    l.[fd] ↦ #l_state ∗ l_state ↦□ state ∗
+    l.[fd] ↦ #l_state ∗ l_state ↦□ (state : val) ∗
     rcfd_lstate_auth γ lstate ∗
     match lstate with
     | RcfdLstateOpen =>
         ∃ q qs,
-        ⌜ops = size qs ∧ set_fold Qp.add q qs = 1%Qp ∧ state = &&Open fd⌝ ∗
+        ⌜ops = size qs ∧ set_fold Qp.add q qs = 1%Qp ∧ state = RcfdStateOpen fd⌝ ∗
         rcfd_tokens_auth γ qs ∗
         unix_fd_model fd (DfracOwn q) chars
     | RcfdLstateClosingUsers =>
         ∃ q qs fn,
-        ⌜ops = size qs ∧ 0 < size qs ∧ set_fold Qp.add q qs = 1%Qp ∧ state = &&Closing fn⌝ ∗
+        ⌜ops = size qs ∧ 0 < size qs ∧ set_fold Qp.add q qs = 1%Qp ∧ state = RcfdStateClosing fn⌝ ∗
         rcfd_tokens_auth γ qs ∗
         unix_fd_model fd (DfracOwn q) chars ∗
         (unix_fd_model fd (DfracOwn 1) chars -∗ WP fn #() {{ res, ⌜res = #()⌝ }})
     | RcfdLstateClosingNoUsers =>
         ∃ fn,
-        ⌜state = &&Closing fn⌝ ∗
+        ⌜state = RcfdStateClosing fn⌝ ∗
         WP fn #() {{ res, ⌜res = #()⌝ }}
     end.
   Definition rcfd_inv t fd chars : iProp Σ :=
@@ -347,21 +374,28 @@ Section rcfd_G.
     ⊢ |==> ∃ γ_tokens,
       rcfd_tokens_auth' γ_tokens ∅.
   Proof.
-    apply auth_dgset_alloc.
+    apply auth_gmultiset_alloc.
   Qed.
   #[local] Lemma rcfd_tokens_elem_of γ qs q :
     rcfd_tokens_auth γ qs -∗
     rcfd_tokens_frag γ q -∗
     ⌜q ∈ qs⌝.
   Proof.
-    apply auth_dgset_elem_of.
+    apply auth_gmultiset_elem_of.
+  Qed.
+  #[local] Lemma rcfd_tokens_update_alloc {γ qs} q :
+    rcfd_tokens_auth γ qs ⊢ |==>
+      rcfd_tokens_auth γ (qs ⊎ {[+q+]}) ∗
+      rcfd_tokens_frag γ q.
+  Proof.
+    apply auth_gmultiset_update_alloc_singleton.
   Qed.
   #[local] Lemma rcfd_tokens_update_dealloc γ qs q :
     rcfd_tokens_auth γ qs -∗
     rcfd_tokens_frag γ q ==∗
-    rcfd_tokens_auth γ (qs ∖ {[q]}).
+    rcfd_tokens_auth γ (qs ∖ {[+q+]}).
   Proof.
-    apply auth_dgset_update_dealloc.
+    apply auth_gmultiset_update_dealloc.
   Qed.
 
   #[local] Lemma rcfd_lstate_alloc :
@@ -446,14 +480,16 @@ Section rcfd_G.
     |}.
     iMod (meta_set _ _ γ with "Hmeta") as "Hmeta"; first done.
     iApply "HΦ". iExists l, γ. iStep 2.
-    iApply inv_alloc. iExists 0, l_state, (&&Open fd), RcfdLstateOpen. iStep 5. iExists 1%Qp, ∅. iSteps.
+    iApply inv_alloc. iExists (RcfdStateOpen fd). iStep 5. iExists 1%Qp, ∅. iSteps.
   Qed.
 
-  #[local] Lemma rcfd_put_spec' l γ fd chars q :
+  #[local] Lemma rcfd_put_spec' l γ fd chars :
     {{{
       inv nroot (rcfd_inv_inner l γ fd chars) ∗
-      ( rcfd_tokens_frag γ q ∗
-        unix_fd_model fd (DfracOwn q) chars
+      ( ( ∃ q,
+          rcfd_tokens_frag γ q ∗
+          unix_fd_model fd (DfracOwn q) chars
+        )
       ∨ rcfd_lstate_lb γ RcfdLstateClosingNoUsers
       )
     }}}
@@ -467,58 +503,59 @@ Section rcfd_G.
     wp_rec. wp_pures.
 
     wp_bind (FAA _ _).
-    iInv "Hinv" as "(%ops1 & %l_state1 & %state1 & %lstate1 & Hops1 & Hfd1 & Hstate1 & Hlstate_auth & Hlstate1)".
+    iInv "Hinv" as "(%state1 & %lstate1 & %ops1 & %l_state1 & Hops1 & Hfd1 & Hstate1 & Hlstate_auth & Hlstate1)".
     wp_faa.
     iSplitR "HΦ".
-    { iDestruct "H" as "[(Htokens_frag & Hmodel) | #Hlstate_lb]".
+    { iDestruct "H" as "[(%q & Htokens_frag & Hmodel) | #Hlstate_lb]".
       - destruct lstate1.
         + iDestruct "Hlstate1" as "(%q' & %qs & (-> & %Hqs & ->) & Htokens_auth & Hmodel')".
           iDestruct (rcfd_tokens_elem_of with "Htokens_auth Htokens_frag") as %Hq.
-          iStep 4. iExists (q + q')%Qp, (qs ∖ {[q]}). iSplitR; last iSplitR "Hmodel Hmodel'".
+          iExists (RcfdStateOpen _). iStep 4. iExists (q + q')%Qp, (qs ∖ {[+q+]}). iSplitR; last iSplitR "Hmodel Hmodel'".
           * iSteps; iPureIntro.
-            -- assert (qs ≢ ∅) as Hqs_size%size_non_empty_iff by set_solver.
-               rewrite size_difference; last set_solver. rewrite size_singleton. lia.
-            -- rewrite (union_difference_singleton_L q qs) // set_fold_disj_union in Hqs; last set_solver.
-               rewrite set_fold_singleton // in Hqs.
+            -- assert (qs ≠ ∅) as Hqs_size%gmultiset_size_non_empty_iff by multiset_solver.
+               rewrite gmultiset_size_difference; last multiset_solver.
+               rewrite gmultiset_size_singleton. lia.
+            -- rewrite (gmultiset_disj_union_difference' q qs) // gmultiset_set_fold_disj_union gmultiset_set_fold_singleton // in Hqs.
           * iMod (rcfd_tokens_update_dealloc with "Htokens_auth Htokens_frag") as "$". iSteps.
           * iCombine "Hmodel Hmodel'" as "$". iSteps.
         + iDestruct "Hlstate1" as "(%q' & %qs & %fn1 & (-> & %Hqs_size & %Hqs & ->) & Htokens_auth & Hmodel' & Hfn1)".
           iDestruct (rcfd_tokens_elem_of with "Htokens_auth Htokens_frag") as %Hq.
           destruct (decide (size qs = 1)) as [Hqs_size' | Hqs_size'].
-          * apply size_1_elem_of in Hqs_size' as (q_ & ->%leibniz_equiv). rewrite set_fold_singleton in Hqs.
-            apply elem_of_singleton in Hq as <-.
+          * apply gmultiset_size_1_elem_of in Hqs_size' as (q_ & ->%leibniz_equiv). rewrite gmultiset_set_fold_singleton in Hqs.
+            apply gmultiset_elem_of_singleton in Hq as <-.
             iMod (rcfd_tokens_update_dealloc with "Htokens_auth Htokens_frag") as "Htokens_auth".
-            assert ({[q]} ∖ {[q]} = ∅) as -> by set_solver.
+            rewrite gmultiset_difference_diag.
             iMod (rcfd_lstate_update RcfdLstateClosingNoUsers with "Hlstate_auth") as "Hlstate_auth"; first done.
             iCombine "Hmodel Hmodel'" as "Hmodel". rewrite Hqs. iDestruct ("Hfn1" with "Hmodel") as "Hfn1".
-            iStep 5. done.
+            iExists (RcfdStateClosing _). iStep 5. done.
           * iMod (rcfd_tokens_update_dealloc with "Htokens_auth Htokens_frag") as "Htokens_auth".
             iCombine "Hmodel Hmodel'" as "Hmodel".
-            iStep 4. iExists (q + q')%Qp, (qs ∖ {[q]}), _. iSteps; iPureIntro.
-            -- rewrite size_difference; last set_solver. rewrite size_singleton. lia.
-            -- rewrite size_difference; last set_solver. rewrite size_singleton. lia.
-            -- rewrite (union_difference_singleton_L q qs) // set_fold_disj_union in Hqs; last set_solver.
-               rewrite set_fold_singleton // in Hqs.
+            iExists (RcfdStateClosing _). iStep 4. iExists (q + q')%Qp, (qs ∖ {[+q+]}). iSteps; iPureIntro.
+            -- rewrite gmultiset_size_difference; last multiset_solver.
+               rewrite gmultiset_size_singleton. lia.
+            -- rewrite gmultiset_size_difference; last multiset_solver.
+               rewrite gmultiset_size_singleton. lia.
+            -- rewrite (gmultiset_disj_union_difference' q qs) // gmultiset_set_fold_disj_union gmultiset_set_fold_singleton // in Hqs.
         + iDestruct "Hlstate1" as "(%fn1 & -> & Hfn1)".
-          iStep 5. done.
+          iExists (RcfdStateClosing _). iStep 5. done.
       - iDestruct (rcfd_lstate_valid_closing_no_users with "Hlstate_auth Hlstate_lb") as %->.
-        iDestruct "Hlstate1" as "(%fn & -> & Hfn)".
-        iStep 5. done.
+        iDestruct "Hlstate1" as "(%fn1 & -> & Hfn1)".
+        iExists (RcfdStateClosing _). iStep 5. done.
     }
     iModIntro. clear.
 
     wp_pures. destruct (decide (ops1 = 1)) as [-> | Hops]; wp_pures; last iSteps.
 
     wp_bind (!_)%E.
-    iInv "Hinv" as "(%ops2 & %l_state2 & %state2 & %lstate2 & Hops2 & Hfd2 & #Hstate2 & Hlstate_auth & Hlstate2)".
+    iInv "Hinv" as "(%state2 & %lstate2 & %ops2 & %l_state2 & Hops2 & Hfd2 & #Hstate2 & Hlstate_auth & Hlstate2)".
     wp_load.
     destruct (decide (lstate2 = RcfdLstateOpen)) as [-> | Hlstate2].
 
     - iDestruct "Hlstate2" as "(%q & %qs & (-> & %Hqs & ->) & Htokens_auth & Hmodel)".
-      iSplitR "HΦ"; first iSteps.
+      iSplitR "HΦ". { iExists (RcfdStateOpen _). iSteps. }
       iSteps.
 
-    - iAssert (∃ fn2, ⌜state2 = &&Closing fn2⌝ ∗ rcfd_lstate_lb γ RcfdLstateClosingUsers)%I as "(%fn2 & -> & #Hlstate_lb)".
+    - iAssert (∃ fn2, ⌜state2 = RcfdStateClosing fn2⌝ ∗ rcfd_lstate_lb γ RcfdLstateClosingUsers)%I as "(%fn2 & -> & #Hlstate_lb)".
       { destruct lstate2; first done.
         - iDestruct "Hlstate2" as "(%q & %qs & %fn2 & (_ & _ & _ & ->) & _)".
           iDestruct (rcfd_lstate_lb_get with "Hlstate_auth") as "$".
@@ -528,27 +565,27 @@ Section rcfd_G.
           iDestruct (rcfd_lstate_lb_mono RcfdLstateClosingUsers with "Hlstate_lb") as "Hlstate_lb"; first done.
           iSteps.
       }
-      iSplitR "HΦ"; first iSteps.
+      iSplitR "HΦ". { iExists (RcfdStateClosing _). iSteps. }
       iModIntro. clear.
 
       wp_load. wp_pures.
 
       wp_bind (!_)%E.
-      iInv "Hinv" as "(%ops3 & %l_state3 & %state3 & %lstate3 & Hops3 & Hfd3 & #Hstate3 & Hlstate_auth & Hlstate3)".
+      iInv "Hinv" as "(%state3 & %lstate3 & %ops3 & %l_state3 & Hops3 & Hfd3 & #Hstate3 & Hlstate_auth & Hlstate3)".
       wp_load.
       iDestruct (rcfd_lstate_valid_closing_users with "Hlstate_auth Hlstate_lb") as %[-> | ->].
 
       + iDestruct "Hlstate3" as "(%q & %qs & %fn3 & (-> & %Hqs_size & %Hqs & ->) & Htokens_auth & Hmodel & Hfn3)".
-        iSplitR "HΦ"; first iSteps.
+        iSplitR "HΦ". { iExists (RcfdStateClosing _). iSteps. }
         iModIntro. clear- Hqs_size.
 
         wp_pures. rewrite bool_decide_eq_true_2; last lia. wp_pures.
 
         iSteps.
 
-      + iDestruct "Hlstate3" as "(%fn & -> & Hfn3)".
+      + iDestruct "Hlstate3" as "(%fn3 & -> & Hfn3)".
         iClear "Hlstate_lb". iDestruct (rcfd_lstate_lb_get with "Hlstate_auth") as "#Hlstate_lb".
-        iSplitR "HΦ"; first by iStep 5.
+        iSplitR "HΦ". { iExists (RcfdStateClosing _). iStep 5. done. }
         iModIntro. clear.
 
         wp_pures. case_bool_decide as Hops3; wp_pures; first iSteps.
@@ -556,15 +593,15 @@ Section rcfd_G.
         wp_rec. wp_alloc closed as "Hclosed". wp_pures.
 
         wp_bind (CmpXchg _ _ _).
-        iInv "Hinv" as "(%ops4 & %l_state4 & %state4 & %lstate4 & Hops4 & Hfd4 & #Hstate4 & Hlstate_auth & Hlstate4)".
+        iInv "Hinv" as "(%state4 & %lstate4 & %ops4 & %l_state4 & Hops4 & Hfd4 & #Hstate4 & Hlstate_auth & Hlstate4)".
         wp_cmpxchg as [= <-] | Hcmpxchg; last iSteps.
         iDestruct (rcfd_lstate_valid_closing_no_users with "Hlstate_auth Hlstate_lb") as %->.
         iDestruct "Hlstate4" as "(%fn4 & -> & Hfn4)".
-        iDestruct (mapsto_agree with "Hstate2 Hstate4") as %<-%(inj _).
-        iSplitR "Hfn4 HΦ"; first iSteps.
+        iDestruct (mapsto_agree with "Hstate2 Hstate4") as %[= <-]%(inj _).
+        iSplitR "Hfn4 HΦ". { iExists (RcfdStateClosing _). iSteps. }
         iSteps.
   Qed.
-  Lemma rcfd_put_spec t fd chars q :
+  #[local] Lemma rcfd_put_spec t fd chars q :
     {{{
       rcfd_inv t fd chars ∗
       rcfd_token t q ∗
@@ -599,7 +636,65 @@ Section rcfd_G.
       end
     }}}.
   Proof.
-  Admitted.
+    iIntros "%Φ (%l & %γ & -> & #Hmeta & #Hinv) HΦ".
+
+    wp_rec. wp_pures.
+
+    wp_bind (FAA _ _).
+    iInv "Hinv" as "(%state1 & %lstate1 & %ops1 & %l_state1 & Hops1 & Hfd1 & Hstate1 & Hlstate_auth & Hlstate1)".
+    wp_faa.
+    iAssert (|==>
+      rcfd_inv_inner l γ fd chars ∗
+      ( ( ∃ q,
+          rcfd_tokens_frag γ q ∗
+          unix_fd_model fd (DfracOwn q) chars
+        )
+      ∨ rcfd_lstate_lb γ RcfdLstateClosingNoUsers
+      )
+    )%I with "[- HΦ]" as ">($ & H)".
+    { destruct lstate1.
+      - iDestruct "Hlstate1" as "(%q & %qs & (-> & %Hqs & ->) & Htokens_auth & Hmodel)".
+        iMod (rcfd_tokens_update_alloc (q / 2) with "Htokens_auth") as "(Htokens_auth & Htokens_frag)".
+        iDestruct "Hmodel" as "(Hmodel1 & Hmodel2)".
+        iSplitR "Htokens_frag Hmodel2"; last iSteps.
+        iExists (RcfdStateOpen _). iStep 4. iExists (q / 2)%Qp, (qs ⊎ {[+q / 2+]})%Qp. iSteps; iPureIntro.
+        + rewrite gmultiset_size_disj_union gmultiset_size_singleton. lia.
+        + rewrite (comm (⊎)) gmultiset_set_fold_disj_union gmultiset_set_fold_singleton Qp.div_2 //.
+      - iDestruct "Hlstate1" as "(%q & %qs & %fn1 & (-> & %Hqs_size & %Hqs & ->) & Htokens_auth & Hmodel & Hfn1)".
+        iMod (rcfd_tokens_update_alloc (q / 2) with "Htokens_auth") as "(Htokens_auth & Htokens_frag)".
+        iDestruct "Hmodel" as "(Hmodel1 & Hmodel2)".
+        iSplitR "Htokens_frag Hmodel2"; last iSteps.
+        iExists (RcfdStateClosing _). iStep 4. iExists (q / 2)%Qp, (qs ⊎ {[+q / 2+]})%Qp. iSteps; iPureIntro.
+        + rewrite gmultiset_size_disj_union gmultiset_size_singleton. lia.
+        + rewrite gmultiset_size_disj_union. lia.
+        + rewrite (comm (⊎)) gmultiset_set_fold_disj_union gmultiset_set_fold_singleton Qp.div_2 //.
+      - iDestruct "Hlstate1" as "(%fn1 & -> & Hfn1)".
+        iDestruct (rcfd_lstate_lb_get with "Hlstate_auth") as "#Hlstate_lb".
+        iSplitL; last iSteps.
+        iExists (RcfdStateClosing _). iSteps.
+    }
+    iModIntro. wp_pures. clear.
+
+    wp_bind (!#l.[fd])%E.
+    iInv "Hinv" as "(%state2 & %lstate2 & %ops2 & %l_state2 & Hops2 & Hfd2 & #Hstate2 & Hlstate_auth & Hlstate2)".
+    wp_load.
+    destruct (decide (lstate2 = RcfdLstateOpen)) as [-> | Hlstate2].
+
+    - iDestruct "Hlstate2" as "(%q & %qs & (-> & %Hqs & ->) & Htokens_auth & Hmodel)".
+      iDestruct "H" as "[(%q' & Htokens_frag & Hmodel') | Hlstate_lb]"; last first.
+      { iDestruct (rcfd_lstate_valid_closing_no_users with "Hlstate_auth Hlstate_lb") as %?. done. }
+      iSplitR "Htokens_frag Hmodel' HΦ". { iExists (RcfdStateOpen _). iSteps. }
+      iSteps. iApply ("HΦ" $! (Some _)). iSteps.
+
+    - iAssert ⌜∃ fn2, state2 = RcfdStateClosing fn2⌝%I as %(fn2 & ->).
+      { destruct lstate2; iDecompose "Hlstate2"; iSteps. }
+      iSplitR "H HΦ". { iExists (RcfdStateClosing fn2). iSteps. }
+      iModIntro. clear.
+
+      wp_load.
+      wp_smart_apply (rcfd_put_spec' with "[$Hinv $H]").
+      iSteps. iApply ("HΦ" $! None). iSteps.
+  Qed.
 
   Lemma rcfd_close_spec t fd chars :
     {{{
@@ -610,7 +705,83 @@ Section rcfd_G.
       RET #b; True
     }}}.
   Proof.
-  Admitted.
+    iIntros "%Φ (%l & %γ & -> & #Hmeta & #Hinv) HΦ".
+
+    wp_rec. wp_pures.
+
+    wp_bind (!_)%E.
+    iInv "Hinv" as "(%state1 & %lstate1 & %ops1 & %l_state1 & Hops1 & Hfd1 & #Hstate1 & Hlstate_auth & Hlstate1)".
+    wp_load.
+    destruct (decide (lstate1 = RcfdLstateOpen)) as [-> | Hlstate1].
+
+    - iDestruct "Hlstate1" as "(%q & %qs & (-> & %Hqs & ->) & Htokens_auth & Hmodel)".
+      iSplitR "HΦ". { iExists (RcfdStateOpen _). iSteps. }
+      iModIntro. clear.
+
+      wp_load.
+      wp_alloc l_state as "Hstate". iMod (mapsto_persist with "Hstate") as "#Hstate".
+      wp_pures.
+
+      wp_bind (CmpXchg _ _ _).
+      iInv "Hinv" as "(%state2 & %lstate2 & %ops2 & %l_state2 & Hops2 & Hfd2 & #Hstate2 & Hlstate_auth & Hlstate2)".
+      wp_cmpxchg as [= <-] | Hcmpxchg; last iSteps.
+      iDestruct (mapsto_agree with "Hstate1 Hstate2") as %[= <-]%(inj _).
+      destruct (decide (lstate2 = RcfdLstateOpen)) as [-> | Hlstate2]; last first.
+      { destruct lstate2; iDecompose "Hlstate2"; iSteps. }
+      iDestruct "Hlstate2" as "(%q & %qs & (-> & %Hqs & _) & Htokens_auth & Hmodel)".
+      iMod (rcfd_lstate_update RcfdLstateClosingUsers with "Hlstate_auth") as "Hlstate_auth"; first done.
+      iDestruct (rcfd_lstate_lb_get with "Hlstate_auth") as "#Hlstate_lb".
+      iSplitR "HΦ".
+      { destruct (decide (size qs = 0)) as [Hqs_size | Hqs_size].
+        - apply gmultiset_size_empty_iff in Hqs_size as ->.
+          rewrite gmultiset_set_fold_empty in Hqs. rewrite {}Hqs.
+          iMod (rcfd_lstate_update RcfdLstateClosingNoUsers with "Hlstate_auth") as "Hlstate_auth"; first done.
+          iExists (RcfdStateClosing _). iSteps. iModIntro.
+          wp_apply (unix_close_spec with "[$]").
+          iSteps.
+        - iExists (RcfdStateClosing _). iSteps. iModIntro.
+          wp_apply (unix_close_spec with "[$]").
+          iSteps.
+      }
+      iModIntro. clear.
+
+      wp_pures.
+
+      wp_bind (!_)%E.
+      iInv "Hinv" as "(%state3 & %lstate3 & %ops3 & %l_state3 & Hops3 & Hfd3 & #Hstate3 & Hlstate_auth & Hlstate3)".
+      wp_load.
+      destruct (decide (ops3 = 0)) as [-> | Hops3]; last iSteps.
+      iDestruct (rcfd_lstate_valid_closing_users with "Hlstate_auth Hlstate_lb") as %[-> | ->].
+      { iDestruct "Hlstate3" as "(%q & %qs & %fn3 & (% & % & _) & _)". lia. }
+      iDestruct "Hlstate3" as "(%fn3 & -> & Hfn3)".
+      iClear "Hlstate_lb". iDestruct (rcfd_lstate_lb_get with "Hlstate_auth") as "#Hlstate_lb".
+      iSplitR "HΦ". { iExists (RcfdStateClosing _). iStep 5. done. }
+      iModIntro. clear.
+
+      wp_pures.
+
+      wp_rec. wp_alloc closed as "Hclosed". wp_pures.
+
+      wp_bind (CmpXchg _ _ _).
+      iInv "Hinv" as "(%state4 & %lstate4 & %ops4 & %l_state4 & Hops4 & Hfd4 & #Hstate4 & Hlstate_auth & Hlstate4)".
+      wp_cmpxchg as [= <-] | Hcmpxchg; last iSteps.
+      iDestruct (rcfd_lstate_valid_closing_no_users with "Hlstate_auth Hlstate_lb") as %->.
+      iDestruct "Hlstate4" as "(%fn4 & -> & Hfn4)".
+      iDestruct (mapsto_agree with "Hstate Hstate4") as %Hfn4. simpl in Hfn4. apply (inj _) in Hfn4 as <-.
+      iSplitR "Hfn4 HΦ". { iExists (RcfdStateClosing _). iSteps. }
+      iModIntro. clear.
+
+      do 2 wp_pure.
+      wp_apply (wp_wand with "Hfn4").
+      iSteps.
+
+    - iAssert ⌜∃ fn1, state1 = RcfdStateClosing fn1⌝%I as %(fn1 & ->).
+      { destruct lstate1; iDecompose "Hlstate1"; iSteps. }
+      iSplitR "HΦ". { iExists (RcfdStateClosing _). iSteps. }
+      iModIntro. clear.
+
+      iSteps.
+  Qed.
 
   Lemma rcfd_use_spec Ψ t fd chars (closed open : val) :
     {{{
@@ -657,16 +828,9 @@ Section rcfd_G.
     iIntros "%Φ (%l & %γ & -> & #Hmeta & #Hinv) HΦ".
     wp_rec. wp_pures.
     wp_bind (!#l.[fd])%E.
-    iInv "Hinv" as "(%ops & %l_state & %state & %lstate & Hops & Hfd & #Hstate & Hlstate_auth & Hlstate)".
+    iInv "Hinv" as "(%state & %lstate & %ops & %l_state & Hops & Hfd & #Hstate & Hlstate_auth & Hlstate)".
     wp_load.
-    destruct lstate.
-    - iDestruct "Hlstate" as "(%q & %qs & (-> & %Hqs & ->) & Htokens_auth & Hmodel)".
-      iSteps.
-    - iDestruct "Hlstate" as "(%q & %qs & %fn & (-> & %Hqs_size & %Hqs & ->) & Htokens_auth & Hmodel & Hfn)".
-      iSplitR "HΦ"; first iSteps.
-      iSteps.
-    - iDestruct "Hlstate" as "(%fn & -> & Hfn)".
-      iSteps.
+    iSteps. destruct state; iSteps.
   Qed.
 
   Lemma rcfd_peek_spec t fd chars :
@@ -682,21 +846,22 @@ Section rcfd_G.
     iIntros "%Φ (%l & %γ & -> & #Hmeta & #Hinv) HΦ".
     wp_rec. wp_pures.
     wp_bind (!#l.[fd])%E.
-    iInv "Hinv" as "(%ops & %l_state & %state & %lstate & Hops & Hfd & #Hstate & Hlstate_auth & Hlstate)".
+    iInv "Hinv" as "(%state & %lstate & %ops & %l_state & Hops & Hfd & #Hstate & Hlstate_auth & Hlstate)".
     wp_load.
     destruct lstate.
     - iDestruct "Hlstate" as "(%q & %qs & (-> & %Hqs & ->) & Htokens_auth & Hmodel)".
+      iSplitR "HΦ". { iExists (RcfdStateOpen _). iSteps. }
       iSteps.
     - iDestruct "Hlstate" as "(%q & %qs & %fn & (-> & %Hqs_size & %Hqs & ->) & Htokens_auth & Hmodel & Hfn)".
-      iSplitR "HΦ"; first iSteps.
+      iSplitR "HΦ". { iExists (RcfdStateClosing _). iSteps. }
       iSteps.
     - iDestruct "Hlstate" as "(%fn & -> & Hfn)".
+      iSplitR "HΦ". { iExists (RcfdStateClosing _). iStep 5. done. }
       iSteps.
   Qed.
 End rcfd_G.
 
 #[global] Opaque rcfd_make.
-#[global] Opaque rcfd_put.
 #[global] Opaque rcfd_get.
 #[global] Opaque rcfd_close.
 #[global] Opaque rcfd_use.
